fix high-level representation of bignum

specs/experimental/rsapss/high-level/Spec.Bignum.Basic.fst
@@ -26,25 +26,30 @@ let bn_cast_gt #n m b = bn #m b
 
 val lemma_bn_add:#n:size_pos -> #m:size_pos{n >= m} -> a:bignum n -> b:bignum m -> Lemma
   (bn_v a + bn_v b < pow2 (n + 1))
-let lemma_bn_add #n #m a b = admit()
+let lemma_bn_add #n #m a b =
+  pow2_le_compat n m;
+  assert (bn_v a + bn_v b < pow2 n + pow2 n);
+  pow2_double_sum n
 
 let bn_add #n #m a b =
   lemma_bn_add #n #m a b;
+  assert (a + b < pow2 (n + 1));
   let res = (a + b) % pow2 n in
   let c = (a + b) / pow2 n in
-  assume (c < pow2 1);
+  lemma_div_lt (a + b) (n + 1) n;
   (u8 c, bn #n res)
 
 let bn_add_carry #n #m a b =
   let res = a + b in
-  assume (res < pow2 (n + 1));
+  lemma_bn_add #n #m a b;
   bn res
 
 let bn_sub #n #m a b = a - b
 
 val lemma_bn_mul:#n:size_pos -> #m:size_pos -> a:bignum n -> b:bignum m -> Lemma
   (bn_v a * bn_v b < pow2 (n + m))
-let lemma_bn_mul #n #m a b = admit()
+let lemma_bn_mul #n #m a b =
+  pow2_plus n m
 
 let bn_mul #n #m a b =
   lemma_bn_mul #n #m a b;
@@ -64,23 +69,47 @@ let bn_from_u64 c = bn #64 (uint_to_nat c)
 
 let bn_is_less #n #m x y = x < y
 
-val lemma_bn_lshift_mul_add:#n:size_pos -> #m:size_pos -> x:bignum n -> i:size_nat -> y:bignum 64 -> z:bignum m -> Lemma
-  (bn_v x * (pow2 i) * bn_v y + bn_v z < pow2 (m + 1))
-let lemma_bn_lshift_mul_add #n #m x i y z = admit()
+val lemma_bn_lshift_mul_add:
+  #n:size_pos -> #m:size_pos -> x:bignum n -> i:size_nat -> y:bignum 64 -> z:bignum m -> Lemma
+  (requires (n + i + 64 <= m))
+  (ensures (bn_v x * pow2 i * bn_v y + bn_v z < pow2 (m + 1)))
+  #reset-options "--z3rlimit 30 --max_fuel 0"
+let lemma_bn_lshift_mul_add #n #m x i y z =
+  assert (bn_v x * pow2 i * bn_v y < pow2 n * pow2 i * pow2 64);
+  pow2_plus n i;
+  pow2_plus (n + i) 64;
+  assert (bn_v x * pow2 i * bn_v y + bn_v z < pow2 (n + i + 64) + pow2 m);
+  pow2_le_compat m (n + i + 64);
+  pow2_double_sum m
 
 let bn_lshift_mul_add #n #m x i y z =
   lemma_bn_lshift_mul_add #n #m x i y z;
-  let res = x * (pow2 i) * y + z in
+  let res = x * pow2 i * y + z in
+  assert (res < pow2 (m + 1));
   let r = res % pow2 m in
   let c = res / pow2 m in
-  assume (c < pow2 1);
+  lemma_div_lt res (m + 1) m;
   (u8 c, bn #m r)
 
+val lemma_bn_lshift_add:
+  #n:size_pos -> #m:size_pos -> x:bignum n -> i:size_nat -> z:bignum m -> Lemma
+  (requires (n + i <= m))
+  (ensures (bn_v x * pow2 i + bn_v z < pow2 (m + 1)))
+  #reset-options "--z3rlimit 30 --max_fuel 0"
+let lemma_bn_lshift_add #n #m x i z =
+  assert (bn_v x * pow2 i < pow2 n * pow2 i);
+  pow2_plus n i;
+  assert (bn_v x * pow2 i+ bn_v z < pow2 (n + i) + pow2 m);
+  pow2_le_compat m (n + i);
+  pow2_double_sum m
+
 let bn_lshift_add #n #m x i z =
-  let res = x * (pow2 i) + z in
+  lemma_bn_lshift_add #n #m x i z;
+  let res = x * pow2 i + z in
+  assert (res < pow2 (m + 1));
   let r = res % pow2 m in
   let c = res / pow2 m in
-  assume (c < pow2 1);
+  lemma_div_lt res (m + 1) m;
   (u8 c, bn #m r)
 
 let bn_from_bytes_be #bBytes b =
