specs/experimental/rsapss/Spec.Bignum.Basic.fsti
@@ -3,24 +3,6 @@ module Spec.Bignum.Basic
 open FStar.Mul
 open Spec.Lib.IntTypes
 open Spec.Lib.IntSeq
-open Spec.Lib.RawIntTypes
-
-(*
-val bignum:Type0
-val bn_v:bignum -> GTot nat
-val bn: n:nat -> b:bignum{bn_v b == n}
-val bn_add: a:bignum -> b:bignum -> c:bignum{bn_v c == bn_v a + bn_v b}
-val bn_mul: a:bignum -> b:bignum -> c:bignum{bn_v c == bn_v a * bn_v b}
-val bn_sub: a:bignum -> b:bignum{bn_v a > bn_v b} -> c:bignum{bn_v c == bn_v a - bn_v b}
-
-val bn_get_bit: b:bignum -> i:size_nat -> c:nat{c == 0 \/ c == 1}
-val bn_get_bits: b:bignum -> i:size_nat{i % 64 == 0} -> j:size_nat{i <= j /\ j % 64 == 0} -> c:bignum{bn_v c < pow2 (j - i) /\ bn_v c == (bn_v b / pow2 i) % pow2 (j - i) }
-val bn_rshift:b:bignum -> i:size_nat{i % 64 == 0} -> c:bignum{bn_v c == bn_v b / pow2 i}
-
-val bn_is_less:a:bignum -> b:bignum -> c:bool{c == true ==> a < b}
-
-val bn_lshift_mul_add:x:bignum -> i:size_nat -> y:bignum{bn_v y < pow2 64} -> z:bignum -> c:bignum{bn_v c == bn_v x * (pow2 i) * bn_v y + bn_v z}
-*)
 
 #reset-options "--z3rlimit 50 --max_fuel 0"
 let blocks (x:size_nat) (m:size_nat{m > 0}): (r:size_nat{x <= m * r}) =
@@ -50,15 +32,15 @@ val bn_sub:#n:size_pos -> #m:size_pos -> a:bignum n -> b:bignum m {bn_v a >= bn_
 val bn_mul:#n:size_pos -> #m:size_pos{n + m < max_size_t} -> a:bignum n -> b:bignum m -> c:bignum (n + m){bn_v c == bn_v a * bn_v b}
 
 val bn_get_bit:#n:size_pos -> b:bignum n -> i:size_nat{i < n} -> c:nat{(c == 0 \/ c == 1) /\ c == (bn_v b / pow2 i) % 2}
-val bn_get_bits:#n:size_pos -> b:bignum n -> i:size_nat{i < n /\ i % 64 == 0} -> j:size_pos{i < j /\ (j % 64 == 0 /\ j <= n) \/ (j = n)} -> c:bignum (j - i){bn_v c == (bn_v b / pow2 i) % pow2 (j - i)}
+val bn_get_bits:#n:size_pos -> b:bignum n -> i:size_nat{i < n /\ i % 64 == 0} -> j:size_pos{i < j /\ (j % 64 == 0 /\ j <= n) \/ j = n} -> c:bignum (j - i){bn_v c == (bn_v b / pow2 i) % pow2 (j - i)}
 val bn_rshift:#n:size_pos -> b:bignum n -> i:size_pos{i < n /\ i % 64 == 0} -> c:bignum (n - i){bn_v c == bn_v b / pow2 i}
 
 val bn_to_u64:b:bignum 64 -> c:uint64{uint_v c == bn_v b}
 val bn_from_u64:c:uint64 -> b:bignum 64{uint_v c == bn_v b}
 
-val bn_is_less:#n:size_pos -> #m:size_pos -> a:bignum n -> b:bignum m -> c:bool{if (c) then bn_v a < bn_v b else bn_v a >= bn_v b}
+val bn_is_less:#n:size_pos -> #m:size_pos -> a:bignum n -> b:bignum m -> c:bool{if c then bn_v a < bn_v b else bn_v a >= bn_v b}
 
-val bn_lshift_mul_add:#n:size_pos -> #m:size_pos{n <= m} -> x:bignum n -> i:size_nat{n + 1 + i <= m} -> y:bignum 64 -> z:bignum m -> Pure (tuple2 carry (bignum m))
+val bn_lshift_mul_add:#n:size_pos -> #m:size_pos{n <= m} -> x:bignum n -> i:size_nat{n + i + 64 <= m} -> y:bignum 64 -> z:bignum m -> Pure (tuple2 carry (bignum m))
   (requires (True))
   (ensures (fun (c, res) -> bn_v res + uint_v c * pow2 m == bn_v x * (pow2 i) * bn_v y + bn_v z))
 
@@ -67,7 +49,6 @@ val bn_lshift_add:#n:size_pos -> #m:size_pos{n <= m} -> x:bignum n -> i:size_nat
   (ensures (fun (c, res) -> bn_v res + uint_v c * pow2 m == bn_v x * (pow2 i) + bn_v z))
 
 val bn_from_bytes_be:#bBytes:size_pos{8 * bBytes < max_size_t} -> b:lbytes bBytes -> Tot (n:bignum (8 * bBytes){bn_v n == nat_from_bytes_be b})
-
 val bn_to_bytes_be: #bBits:size_pos -> n:bignum bBits ->  Tot (b:lbytes (blocks bBits 8) {bn_v n == nat_from_bytes_be b})
 
 val bn_pow2_r_mod:#nBits:size_pos -> n:bignum nBits{bn_v n > 0} -> r:size_pos -> c:bignum nBits{bn_v c == (pow2 r) % (bn_v n)}
